operators semantic preservation proof complete (few operators work for int32 only)

compiler_test/div1.c
@@ -1,0 +1,11 @@
+#include <stdio.h>
+
+short div(short x, short y) {
+        return  x / y;
+}
+
+int main() {
+        short r = div(8, 2);
+        printf("%d", r); 
+        return 0;
+}
